src/Commutable.v
@@ -1,0 +1,175 @@
+Require Import Bool List String Peano_dec.
+Require Import Common ListSupport FMap Syntax Semantics StepM StepT SemFacts.
+Require Import Topology Serial SerialFacts Reduction.
+
+Set Implicit Arguments.
+
+Definition ruleOfL {MsgT} (lbl: RLabel MsgT): option Rule :=
+  match lbl with
+  | RlblInt rule _ _ => Some rule
+  | _ => None
+  end.
+
+Fixpoint rulesOfH (hst: MHistory) :=
+  match hst with
+  | nil => nil
+  | lbl :: hst' => (ruleOfL lbl) ::> (rulesOfH hst')
+  end.
+
+(* Definition insOfL {MsgT} (lbl: RLabel MsgT): list (Id MsgT) := *)
+(*   match lbl with *)
+(*   | RlblInt _ ins _ => ins *)
+(*   | RlblOuts outs => outs *)
+(*   | _ => nil *)
+(*   end. *)
+
+(* Definition outsOfL {MsgT} (lbl: RLabel MsgT): list (Id MsgT) := *)
+(*   match lbl with *)
+(*   | RlblIns ins => ins *)
+(*   | RlblInt _ _ outs => outs *)
+(*   | _ => nil *)
+(*   end. *)
+
+(* Fixpoint insOfH (hst: MHistory) := *)
+(*   match hst with *)
+(*   | nil => nil *)
+(*   | lbl :: hst' => insOfH hst' ++ insOfL lbl *)
+(*   end. *)
+
+(* Fixpoint outsOfH (hst: MHistory) := *)
+(*   match hst with *)
+(*   | nil => nil *)
+(*   | lbl :: hst' => outsOfH hst' ++ outsOfL lbl *)
+(*   end. *)
+
+(** TODO: need to check whether the disjointness between [ins1] and [ins2] 
+ * (or [outs1] and [outs2]) is required. *)
+Definition NonConflictingR (rule1 rule2: Rule) :=
+  forall post1 porq1 ins1 nost1 norq1 outs1 ins2,
+    rule_precond rule1 post1 porq1 ins1 ->
+    rule_trs rule1 post1 porq1 ins1 = (nost1, norq1, outs1) ->
+    rule_precond rule2 nost1 norq1 ins2 ->
+    (* 1) Precondition of [rule2] holds if the one of [rule1] holds. *)
+    rule_precond rule2 post1 porq1 ins2 /\
+    forall nost2 norq2 outs2,
+      rule_trs rule2 post1 porq1 ins2 = (nost2, norq2, outs2) ->
+      (* 2) Precondition of [rule1] holds after a transition by [rule2]. *)
+      rule_precond rule1 nost2 norq2 ins1 /\
+      (* 3) Transitions by [rule1; rule2] and [rule2; rule1] are same. *)
+      fst (rule_trs rule2 nost1 norq1 ins2) =
+      fst (rule_trs rule1 nost2 norq2 ins1).
+
+Definition NonConflictingH (hst1 hst2: MHistory) :=
+  forall rule1 rule2,
+    In rule1 (rulesOfH hst1) ->
+    In rule2 (rulesOfH hst2) ->
+    rule_oidx rule1 = rule_oidx rule2 ->
+    NonConflictingR rule1 rule2.
+
+Definition DiscontinuousI (hst1 hst2: MHistory) :=
+  forall eins1 inits2 ins2 outs2 eouts2,
+    hst1 = [RlblIns eins1] ->
+    Atomic msg_dec inits2 ins2 hst2 outs2 eouts2 ->
+    DisjList eins1 ins2 /\ DisjList (idsOf eins1) (idsOf outs2).
+
+Definition DiscontinuousO (hst1 hst2: MHistory) :=
+  forall inits1 ins1 outs1 eouts1 eouts2,
+    Atomic msg_dec inits1 ins1 hst1 outs1 eouts1 ->
+    hst2 = [RlblOuts eouts2] ->
+    DisjList (idsOf eouts2) (idsOf ins1) /\ DisjList eouts2 outs1.
+
+Definition DiscontinuousA (sys: System) (hst1 hst2: MHistory) :=
+  forall inits1 ins1 outs1 eouts1 inits2 ins2 outs2 eouts2,
+    Atomic msg_dec inits1 ins1 hst1 outs1 eouts1 ->
+    Atomic msg_dec inits2 ins2 hst2 outs2 eouts2 ->
+    DisjList (idsOf ins1) (idsOf ins2) /\
+    DisjList inits1 eouts2 /\
+    DisjList (idsOf outs1) (idsOf outs2).
+
+Definition trsTypeOf (hst: MHistory) :=
+  match hst with
+  | nil => TSlt
+  | lbl :: _ =>
+    match lbl with
+    | RlblEmpty _ => TSlt
+    | RlblIns _ => TIns
+    | RlblOuts _ => TOuts
+    | RlblInt _ _ _ => TInt
+    end
+  end.
+
+Definition DiscontinuousTrsType (tty1 tty2: TrsType) :=
+  match tty1, tty2 with
+  | TSlt, _ => True
+  | _, TSlt => True
+  | TInt, _ => True
+  | _, TInt => True
+  | _, _ => False
+  end.
+
+Definition Discontinuous (sys: System) (hst1 hst2: MHistory) :=
+  DiscontinuousTrsType (trsTypeOf hst1) (trsTypeOf hst2) /\
+  DiscontinuousI hst1 hst2 /\
+  DiscontinuousO hst1 hst2 /\
+  DiscontinuousA sys hst1 hst2.
+
+Lemma nonconflicting_discontinuous_commutable_atomic_sub:
+  forall sys rule1 ins1 outs1 inits2 ins2 hst2 outs2 eouts2,
+    Atomic msg_dec inits2 ins2 hst2 outs2 eouts2 ->
+    (forall rule2,
+        In rule2 (rulesOfH hst2) ->
+        rule_oidx rule1 = rule_oidx rule2 ->
+        NonConflictingR rule1 rule2) ->
+    DisjList (idsOf ins1) (idsOf ins2) ->
+    DisjList ins1 eouts2 ->
+    DisjList (idsOf outs1) (idsOf outs2) ->
+    Reducible sys (hst2 ++ [RlblInt rule1 ins1 outs1])
+              (RlblInt rule1 ins1 outs1 :: hst2).
+Proof.
+  induction 1; simpl; intros.
+Admitted.
+
+Lemma nonconflicting_discontinuous_commutable_atomic:
+  forall sys inits1 ins1 hst1 outs1 eouts1
+         inits2 ins2 hst2 outs2 eouts2,
+    Atomic msg_dec inits1 ins1 hst1 outs1 eouts1 ->
+    Atomic msg_dec inits2 ins2 hst2 outs2 eouts2 ->
+    NonConflictingH hst1 hst2 ->
+    DisjList (idsOf ins1) (idsOf ins2) ->
+    DisjList inits1 eouts2 ->
+    DisjList (idsOf outs1) (idsOf outs2) ->
+    Reducible sys (hst2 ++ hst1) (hst1 ++ hst2).
+Proof.
+Admitted.
+
+Theorem nonconflicting_discontinuous_commutable:
+  forall sys hst1 hst2,
+    STransactional msg_dec hst1 ->
+    STransactional msg_dec hst2 ->
+    NonConflictingH hst1 hst2 ->
+    Discontinuous sys hst1 hst2 ->
+    Reducible sys (hst2 ++ hst1) (hst1 ++ hst2).
+Proof.
+  intros.
+  red in H2; dest.
+  inv H.
+  - apply silent_reducible_2.
+  - inv H0; try (exfalso; auto; fail).
+    + apply silent_reducible_1.
+    + specialize (H3 _ _ _ _ _ eq_refl H); dest.
+      eapply msg_ins_reducible_2; eauto.
+  - inv H0; try (exfalso; auto; fail).
+    + apply silent_reducible_1.
+    + apply msg_outs_reducible_2.
+      eauto using atomic_internal_history.
+  - inv H0.
+    + apply silent_reducible_1.
+    + apply msg_ins_reducible_1.
+      eauto using atomic_internal_history.
+    + specialize (H4 _ _ _ _ _ H6 eq_refl); dest.
+      eapply msg_outs_reducible_1; eauto.
+    + red in H5.
+      specialize (H5 _ _ _ _ _ _ _ _ H6 H); dest.
+      eauto using nonconflicting_discontinuous_commutable_atomic.
+Qed.
+
